src/Sub.v
@@ -34,15 +34,15 @@ Equations STmL {Γ Γ' τ} (s : Sub Γ Γ')
 
 Fixpoint STmExp {Γ Γ' τ} (s : Sub Γ Γ') (e : Exp Γ τ) : Exp Γ' τ :=
   match e with
-  | Constant lit    => Constant lit
-  | Seq exp1 exp2   => Seq (STmExp s exp1) (STmExp s exp2)
-  | Nil             => Nil
-  | Cons x xs       => Cons (STmExp s x) (STmExp s xs)
-  | Let binder body => Let (STmExp s binder) (STmExp (STmL s) body)
+  | Constant lit  => Constant lit
+  | Seq exp1 exp2 => Seq (STmExp s exp1) (STmExp s exp2)
+  | Nil           => Nil
+  | Cons x xs     => Cons (STmExp s x) (STmExp s xs)
+  | Let x body    => Let (STmExp s x) (STmExp (STmL s) body)
 
-  | VAR v     => s _ v
-  | APP e1 e2 => APP (STmExp s e1) (STmExp s e2)
-  | LAM e     => LAM (STmExp (STmL s) e)
+  | VAR v         => s _ v
+  | APP e1 e2     => APP (STmExp s e1) (STmExp s e2)
+  | LAM e         => LAM (STmExp (STmL s) e)
   end.
 
 Definition ScR {Γ Γ' Γ''} (s : Sub Γ' Γ'') (r : Ren Γ Γ') :=
